examples/sbf/verif.v
@@ -80,7 +80,7 @@ Definition Row_regact_insert_apply_spec : func_spec :=
     (fun _ => ValBaseBit (P4Arith.to_loptbool 8%N 1)).
 
 Lemma Row_regact_insert_apply_body :
-  fundef_satisfies_spec am_ge Row_regact_insert_apply_fd nil Row_regact_insert_apply_spec.
+  func_sound am_ge Row_regact_insert_apply_fd nil Row_regact_insert_apply_spec.
 Proof.
   start_function.
   step.
@@ -115,7 +115,7 @@ Definition NoAction_spec : func_spec :=
         (EXT []))).
 
 Lemma NoAction_body :
-  fundef_satisfies_spec ge NoAction_fundef nil NoAction_spec.
+  func_sound ge NoAction_fundef nil NoAction_spec.
 Proof.
   start_function.
   step.
@@ -148,7 +148,7 @@ Definition Row_insert_spec : func_spec :=
         (EXT [row_repr p (row_insert r i)]))).
 
 Lemma Row_insert_body :
-  fundef_satisfies_spec ge Row_insert_fundef nil Row_insert_spec.
+  func_sound ge Row_insert_fundef nil Row_insert_spec.
 Proof.
   start_function.
   unfold row_repr, row_reg_repr.
@@ -185,7 +185,7 @@ Definition Row_regact_query_apply_spec : func_spec :=
     (fun b => ValBaseBit (P4Arith.to_loptbool 8%N b)).
 
 Lemma Row_regact_query_apply_body :
-  fundef_satisfies_spec am_ge Row_regact_query_apply_fd nil Row_regact_query_apply_spec.
+  func_sound am_ge Row_regact_query_apply_fd nil Row_regact_query_apply_spec.
 Proof.
   start_function.
   step.
@@ -241,7 +241,7 @@ Proof.
 Qed.
 
 Lemma Row_query_body :
-  fundef_satisfies_spec ge Row_query_fundef nil Row_query_spec.
+  func_sound ge Row_query_fundef nil Row_query_spec.
 Proof.
   start_function.
   unfold row_repr, row_reg_repr.
@@ -285,7 +285,7 @@ Definition Row_regact_clear_apply_spec : func_spec :=
     (fun _ => ValBaseBit (P4Arith.to_loptbool 8%N 0)).
 
 Lemma Row_regact_clear_apply_body :
-  fundef_satisfies_spec am_ge Row_regact_clear_apply_fd nil Row_regact_clear_apply_spec.
+  func_sound am_ge Row_regact_clear_apply_fd nil Row_regact_clear_apply_spec.
 Proof.
   start_function.
   step.
@@ -328,7 +328,7 @@ Definition Row_clear_spec : func_spec :=
         (EXT [row_repr p (row_clear r i)]))).
 
 Lemma Row_clear_body :
-  fundef_satisfies_spec ge Row_clear_fundef nil Row_clear_spec.
+  func_sound ge Row_clear_fundef nil Row_clear_spec.
 Proof.
   start_function.
   unfold row_repr, row_reg_repr.
@@ -380,7 +380,7 @@ Definition Row_tbl_bloom_spec : func_spec :=
            r)]))))%arg_ret_assr.
 
 Lemma Row_tbl_bloom_body :
-  fundef_satisfies_spec ge Row_tbl_bloom_fundef nil Row_tbl_bloom_spec.
+  func_sound ge Row_tbl_bloom_fundef nil Row_tbl_bloom_spec.
 Proof.
   split. 2 : {
     solve_modifies.
@@ -469,7 +469,7 @@ Definition Row_fundef := Eval compute in
   action list. That can be guaranteed in the lookup and synthesize step. *)
 
 Lemma Row_body :
-  fundef_satisfies_spec ge Row_fundef nil Row_spec.
+  func_sound ge Row_fundef nil Row_spec.
 Proof.
   start_function.
   step.
@@ -518,7 +518,7 @@ Definition Row_tbl_bloom_noop_spec : func_spec :=
         (EXT [row_repr p r]))))%arg_ret_assr.
 
 Lemma Row_tbl_bloom_noop_body :
-  fundef_satisfies_spec ge Row_tbl_bloom_fundef nil Row_tbl_bloom_noop_spec.
+  func_sound ge Row_tbl_bloom_fundef nil Row_tbl_bloom_noop_spec.
 Proof.
   split. 2 : {
     solve_modifies.
@@ -547,7 +547,7 @@ Proof.
 Qed.
 
 Lemma Row_noop_case_body :
-  fundef_satisfies_spec ge Row_fundef nil Row_noop_case_spec.
+  func_sound ge Row_fundef nil Row_noop_case_spec.
 Proof.
   start_function.
   step.
@@ -595,7 +595,7 @@ Definition Row_tbl_bloom_insert_spec : func_spec :=
         (EXT [row_repr p (row_insert r i)]))))%arg_ret_assr.
 
 Lemma Row_tbl_bloom_insert_body :
-  fundef_satisfies_spec ge Row_tbl_bloom_fundef nil Row_tbl_bloom_insert_spec.
+  func_sound ge Row_tbl_bloom_fundef nil Row_tbl_bloom_insert_spec.
 Proof.
   split. 2 : {
     solve_modifies.
@@ -626,7 +626,7 @@ Proof.
 Qed.
 
 Lemma Row_insert_case_body :
-  fundef_satisfies_spec ge Row_fundef nil Row_insert_case_spec.
+  func_sound ge Row_fundef nil Row_insert_case_spec.
 Proof.
   start_function.
   step.
@@ -674,7 +674,7 @@ Definition Row_tbl_bloom_query_spec : func_spec :=
         (EXT [row_repr p r]))))%arg_ret_assr.
 
 Lemma Row_tbl_bloom_query_body :
-  fundef_satisfies_spec ge Row_tbl_bloom_fundef nil Row_tbl_bloom_query_spec.
+  func_sound ge Row_tbl_bloom_fundef nil Row_tbl_bloom_query_spec.
 Proof.
   split. 2 : {
     solve_modifies.
@@ -707,7 +707,7 @@ Proof.
 Qed.
 
 Lemma Row_query_case_body :
-  fundef_satisfies_spec ge Row_fundef nil Row_query_case_spec.
+  func_sound ge Row_fundef nil Row_query_case_spec.
 Proof.
   start_function.
   step.
@@ -755,7 +755,7 @@ Definition Row_tbl_bloom_clear_spec : func_spec :=
         (EXT [row_repr p (row_clear r i)]))))%arg_ret_assr.
 
 Lemma Row_tbl_bloom_clear_body :
-  fundef_satisfies_spec ge Row_tbl_bloom_fundef nil Row_tbl_bloom_clear_spec.
+  func_sound ge Row_tbl_bloom_fundef nil Row_tbl_bloom_clear_spec.
 Proof.
   split. 2 : {
     solve_modifies.
@@ -786,7 +786,7 @@ Proof.
 Qed.
 
 Lemma Row_clear_case_body :
-  fundef_satisfies_spec ge Row_fundef nil Row_clear_case_spec.
+  func_sound ge Row_fundef nil Row_clear_case_spec.
 Proof.
   start_function.
   step.
